proved freeze, removed initial carry step (the correctness proof of that step needs bounds-checker)

src/Arithmetic/Saturated.v
@@ -108,7 +108,7 @@ Module Columns.
             {weight_positive : forall i, weight i > 0}
             {weight_multiples : forall i, weight (S i) mod weight i = 0}
             {weight_divides : forall i : nat, weight (S i) / weight i > 0}
-    (* add_get_carry takes in a number at which to split output *)
+            (* add_get_carry takes in a number at which to split output *)
             {add_get_carry: Z ->Z -> Z -> (Z * Z)}
             {add_get_carry_mod : forall s x y,
                 fst (add_get_carry s x y)  = (x + y) mod s}
@@ -418,27 +418,30 @@ Module Columns.
         rewrite eval_cons_to_nth by omega. nsatz.
     Qed.
 
-    Definition mul_cps {n m} (p q : Z^n) {T} (f : (list Z)^m->T) :=
-      B.Positional.to_associational_cps weight p
-        (fun P => B.Positional.to_associational_cps weight q
-        (fun Q => B.Associational.mul_cps P Q
-        (fun PQ => from_associational_cps m PQ f))).
-
-    Definition add_cps {n} (p q : Z^n) {T} (f : (list Z)^n->T) :=
-      B.Positional.to_associational_cps weight p
-        (fun P => B.Positional.to_associational_cps weight q
-        (fun Q => from_associational_cps n (P++Q) f)).
-
-    Definition sub_cps {n} (p q : Z^n) {T} (f : (list Z)^n->T) :=
-      B.Positional.to_associational_cps weight p
-        (fun P => B.Positional.to_associational_cps weight q
-        (fun Q => from_associational_cps n (P++Q) f)).
-
   End Columns.
+
+  Section Wrappers.
+    Context (weight : nat->Z)
+            {add_get_carry: Z ->Z -> Z -> (Z * Z)}
+            {div modulo : Z -> Z -> Z}.
+
+    Definition add_cps {n} (p q : Z^n) {T} (f : (Z*Z^n)->T) :=
+      B.Positional.to_associational_cps weight p
+        (fun P => B.Positional.to_associational_cps weight q
+        (fun Q => from_associational_cps weight n (P++Q)
+        (fun R => compact_cps (div:=div) (modulo:=modulo) (add_get_carry:=add_get_carry) weight R f))).
+
+    Definition sub_cps {n} (p q : Z^n) {T} (f : (Z*Z^n)->T) :=
+      B.Positional.to_associational_cps weight p
+        (fun P => B.Positional.negate_snd_cps weight q
+        (fun nq => B.Positional.to_associational_cps weight nq
+        (fun Q => from_associational_cps weight n (P++Q)
+        (fun R => compact_cps (div:=div) (modulo:=modulo) (add_get_carry:=add_get_carry) weight R f)))).
+   
+    End Wrappers.
 End Columns.
 Hint Unfold
      Columns.add_cps
-     Columns.mul_cps
      Columns.sub_cps.
 Hint Rewrite
      @Columns.compact_digit_id
@@ -493,8 +496,7 @@ Section Freeze.
 
   Definition conditional_add_cps {n} mask cond (p q : Z^n) {T} (f:_->T) :=
     conditional_mask_cps mask cond q
-    (fun qq => Columns.add_cps weight p qq
-    (fun R => Columns.compact_cps (div:=div) (modulo:=modulo) (add_get_carry:=add_get_carry) weight R f)).
+    (fun qq => Columns.add_cps (div:=div) (modulo:=modulo) (add_get_carry:=add_get_carry) weight p qq f).
   Definition conditional_add {n} mask cond p q :=
     @conditional_add_cps n mask cond p q _ id.
   Lemma conditional_add_id {n} mask cond p q T f:
@@ -509,33 +511,31 @@ Section Freeze.
   
   
   (*
+    The input to [freeze] should be less than 2*m (this can probably
+    be accomplished by a single carry_reduce step, for most moduli).
+
     [freeze] has the following steps:
-    (1) pseudomersenne reduction using [carry_reduce]
-    (2) subtract modulus in a carrying loop (in our framework, this
+    (1) subtract modulus in a carrying loop (in our framework, this
     consists of two steps; [Columns.sub_cps] combines the input p and
     the modulus m such that the ith limb in the output is the list
     [p[i];-m[i]]. We can then call [Columns.compact].)
-    (3) look at the final carry, which should be either 0 or -1. If
+    (2) look at the final carry, which should be either 0 or -1. If
     it's -1, then we add the modulus back in. Otherwise we add 0 for
     constant-timeness.
-    (4) discard the carry after this last addition; it should be 1 if
+    (3) discard the carry after this last addition; it should be 1 if
     the carry in step 3 was -1, so they cancel out.
    *)
-  Definition freeze_cps
-             {n} (mask:Z) (s:Z) (c:list B.limb) (m:Z^n) (p:Z^n)
-             {T} (f : Z^n->T) :=
-    B.Positional.carry_reduce_cps
-      (div:=div) (modulo:=modulo) weight s c p
-      (fun P => Columns.sub_cps weight P m
-      (fun Q => Columns.compact_cps (div:=div) (modulo:=modulo) (add_get_carry:=add_get_carry) weight Q
-      (fun carry_q => conditional_add_cps mask (fst carry_q) (snd carry_q) m
-      (fun carry_r => f (snd carry_r)))))
+  Definition freeze_cps {n} (mask:Z) (m:Z^n) (p:Z^n) {T} (f : Z^n->T) :=
+    Columns.sub_cps (div:=div) (modulo:=modulo)
+                    (add_get_carry:=add_get_carry) weight p m
+      (fun carry_p => conditional_add_cps mask (fst carry_p) (snd carry_p) m
+      (fun carry_r => f (snd carry_r)))
   .
 
-  Definition freeze {n} mask s c m p :=
-    @freeze_cps n mask s c m p _ id.
-  Lemma freeze_id {n} mask s c m p T f:
-    @freeze_cps n mask s c m p T f = f (freeze mask s c m p).
+  Definition freeze {n} mask m p :=
+    @freeze_cps n mask m p _ id.
+  Lemma freeze_id {n} mask m p T f:
+    @freeze_cps n mask m p T f = f (freeze mask m p).
   Proof.
     cbv [freeze_cps freeze]; repeat progress autounfold;
       autorewrite with uncps push_id; reflexivity.
@@ -590,13 +590,17 @@ Section Freeze.
     y0 = y - m ->
     z = y0 mod s ->
     c0 = y0 / s ->
-    c0 <> 0 ->
     z0 = z + (if (dec (c0 = 0)) then 0 else m) ->
     a = z0 mod s ->
     a mod m = y0 mod m.
   Proof.
     clear. intros. subst. break_match.
-    { rewrite Z.add_0_r, Z.mod_mod, !Z.mod_small by omega.
+    { rewrite Z.add_0_r, Z.mod_mod by omega.
+      assert (-(s-c) <= y - (s-c) < s-c) by omega.
+      match goal with H : s <> 0 |- _ =>
+                      rewrite (proj2 (Z.mod_small_iff _ s H))
+                              by (apply Z.div_small_iff; assumption)
+      end.
       reflexivity. }
     { rewrite <-Z.add_mod_l, Z.sub_mod_full.
       rewrite Z.mod_same, Z.sub_0_r, Z.mod_mod by omega.
@@ -604,36 +608,40 @@ Section Freeze.
       by (pose proof (Z.div_small (y - (s-c)) s); omega).
       f_equal. ring. }
   Qed.
-
-  Lemma eval_freeze {n} mask s c m p
-        (n_nonzero:n<>0%nat) (s_nonzero:s<>0)
-        (Hweight : weight (S (pred n)) / weight (pred n) <> 0)
+  
+  Lemma eval_freeze {n} mask c m p
+        (n_nonzero:n<>0%nat)
         (Hmask : Tuple.map (Z.land mask) m = m)
+        (Hc : 0 < B.Associational.eval c < weight n)
         modulus (Hm : B.Positional.eval weight m = Z.pos modulus)
-        (Hsc : Z.pos modulus = s - B.Associational.eval c)
+        (Hp : 0 <= B.Positional.eval weight p < 2*(Z.pos modulus))
+        (Hsc : Z.pos modulus = weight n - B.Associational.eval c)
     :
       mod_eq modulus
-             (B.Positional.eval weight (@freeze n mask s c m p))
+             (B.Positional.eval weight (@freeze n mask m p))
              (B.Positional.eval weight p).
   Proof.
-    cbv [freeze_cps freeze mod_eq conditional_add_cps].
+    cbv [freeze_cps freeze conditional_add_cps].
     repeat progress autounfold.
-    autorewrite with uncps push_id.
+    autorewrite with uncps push_id push_basesystem_eval.
 
-    match goal with |- context [B.Associational.reduce ?s ?c ?p] =>
-                    remember (B.Associational.reduce s c p) as y end.
-    match goal with |- context [fst ?x] =>
-                    remember x as carry_q end.
-    match goal with |- context [conditional_mask ?mask ?cond ?p] =>
-                    remember (conditional_mask mask cond p) as m0 end.
-    match goal with |- context [Columns.compact ?w ?p] =>
-                    remember (Columns.compact w p) as carry_r end.
-    destruct carry_q as [c0 z].
-    destruct carry_r as [c1 a].
-    
-  Admitted.
+    pose proof (weight_nonzero n).
+
+    remember (B.Positional.eval weight p) as y.
+    remember (y + -B.Positional.eval weight m) as y0.
+    rewrite Hm in *.
+
+    transitivity y0; cbv [mod_eq].
+    { eapply (freezeZ (Z.pos modulus) (weight n) (B.Associational.eval c) y y0);
+        try assumption; reflexivity. }
+    { subst y0.
+      assert (Z.pos modulus <> 0) by auto using Z.positive_is_nonzero, Zgt_pos_0.
+      rewrite Z.add_mod by assumption.
+      rewrite Z.mod_opp_l_z by auto using Z.mod_same.
+      rewrite Z.add_0_r, Z.mod_mod by assumption.
+      reflexivity. }
+  Qed.
 End Freeze.
-    
 
   
 (*
